# 2.8.7 $\arctan x$ 与 $\arctan y$ 的和与差

$$
\arctan x + \arctan y = \arctan \frac{x + y}{1 - {xy}}\;\left( {{xy} < 1}\right)  \tag{2.159a}
$$

$$
= \pi  + \arctan \frac{x + y}{1 - {xy}}\;\left( {x > 0,{xy} > 1}\right)  \tag{2.159b}
$$

$$
=  - \pi  + \arctan \frac{x + y}{1 - {xy}}\;\left( {x < 0,{xy} > 1}\right) . \tag{2.159c}
$$

$$
\arctan x - \arctan y = \arctan \frac{x - y}{1 + {xy}}\;\left( {{xy} >  - 1}\right)  \tag{2.160a}
$$

$$
= \pi  + \arctan \frac{x - y}{1 + {xy}}\;\left( {x > 0,{xy} <  - 1}\right)  \tag{2.160b}
$$

$$
=  - \pi  + \arctan \frac{x - y}{1 + {xy}}\;\left( {x < 0,{xy} <  - 1}\right)  \tag{2.160c}
$$
