# 2.8.5 $\arcsin x$ 与 $\arcsin y$ 的和与差

$$
\arcsin x + \arcsin y
$$

$$
= \arcsin \left( {x\sqrt{1 - {y}^{2}} + y\sqrt{1 - {x}^{2}}}\right) \;\left( {{xy} \leq  0\text{ 或 }{x}^{2} + {y}^{2} \leq  1}\right)  \tag{2.155a}
$$

$$
= \pi  - \arcsin \left( {x\sqrt{1 - {y}^{2}} + y\sqrt{1 - {x}^{2}}}\right) \;\left( {x > 0, y > 0,{x}^{2} + {y}^{2} > 1}\right)
$$

(2.155b)

$$
=  - \pi  - \arcsin \left( {x\sqrt{1 - {y}^{2}} + y\sqrt{1 - {x}^{2}}}\right) \;\left( {x < 0, y < 0,{x}^{2} + {y}^{2} > 1}\right) .
$$

(2.155c)

$$
\arcsin x - \arcsin y
$$

$$
= \arcsin \left( {x\sqrt{1 - {y}^{2}} - y\sqrt{1 - {x}^{2}}}\right) \;\left( {{xy} \geq  0\text{ 或 }{x}^{2} + {y}^{2} \leq  1}\right)  \tag{2.156a}
$$

$$
= \pi  - \arcsin \left( {x\sqrt{1 - {y}^{2}} - y\sqrt{1 - {x}^{2}}}\right) \;\left( {x > 0, y < 0,{x}^{2} + {y}^{2} > 1}\right.  \tag{2.156b}
$$

$$
=  - \pi  - \arcsin \left( {x\sqrt{1 - {y}^{2}} - y\sqrt{1 - {x}^{2}}}\right) \;\left( {x < 0, y > 0,{x}^{2} + {y}^{2} > 1}\right) .
$$

(2.156c)
