# 2.8.6 $\arccos x$ 与 $\arccos y$ 的和与差

$$
\arccos x + \arccos y
$$

$$
= \arccos \left( {{xy} - \sqrt{1 - {x}^{2}}\sqrt{1 - {y}^{2}}}\right) \;\left( {x + y \geq  0}\right)  \tag{2.157a}
$$

$$
= {2\pi } - \arccos \left( {{xy} - \sqrt{1 - {x}^{2}}\sqrt{1 - {y}^{2}}}\right) \;\left( {x + y < 0}\right) . \tag{2.157b}
$$

$$
\arccos x - \arccos y
$$

$$
=  - \arccos \left( {{xy} + \sqrt{1 - {x}^{2}}\sqrt{1 - {y}^{2}}}\right) \;\left( {x \geq  y}\right)  \tag{2.158a}
$$

$$
= \arccos \left( {{xy} + \sqrt{1 - {x}^{2}}\sqrt{1 - {y}^{2}}}\right) \;\left( {x < y}\right) . \tag{2.158b}
$$
